\documentclass[11pt,openany]{article}

\input{grad-math-preamble}
\input{tcolorbox}
\input{theorem}
\input{tikz}
\input{grad-math-commands}

\setstretch{1.25}
\begin{document}
\pagenumbering{arabic}
\begin{center}
	\huge\textbf{Advanced Calculus II}\\
	\vspace{0.5em}
	\large{Ji, Yong-hyeon}\\
	\vspace{0.5em}
	\normalsize{\today}\\
\end{center}

\noindent 
We cover the following topics in this note.
\begin{itemize}
	\item Convergence of Sequences
	\item Inequality Rule for Absolute Values
	\item \st{Limit Theorem (Algebraic Property of Limit of Sequence)}
\end{itemize}
\hrule\vspace{12pt}
%Preliminaries:
%\begin{itemize}
%	\item Boundedness, Supremum and Infimum
%	\item Least Upper Bound Property (Completeness Axiom)
%	\item Well-Ordering Principle and Mathematical Induction
%	\item Archimedean Property
%\end{itemize}
%\hrule\vspace{12pt}

\vfill
\defbox[Sequence]{\begin{definition*}
	Let $X\subseteq\R$. A \textbf{sequence} is a function \[
	f:\N\to X(\subseteq\R),\quad n\mapsto f(n):=a_n.
	\] Instead of using function notation $f(n)$, the values of the sequence are denoted by $\set{a_n}_{n=1}^\infty$, where $a_n=f(n)$ is called $n$-th term of the sequence.
\end{definition*}}
\begin{remark*}
A sequence in $X\subseteq\R$ is a function \[
a:\N\to X,\quad n\mapsto a_n,
\] where $a_n\in X$ for all $n\in\N$. We sometimes write \[
\set{a_n},\quad\set{a_n}_{n=1}^\infty,\quad \set{a_n}_{n\in\N},\quad (a_n)_{n\in\N},\quad\ \text{or}\quad \gen{a_n}_{n\in\N}.
\]
\end{remark*}
\defbox[Convergence of Sequence]{\begin{definition*}
	A real sequence $\set{a_n}_{n=1}^\infty(\subseteq\R)$ is said to \textbf{converge} to $L\in\R$ if and only if \[
\forall\varepsilon>0,\ \exists N_\epsilon\in\N\ \text{such that}\ \left[ n\geq N_\epsilon\implies \abs{a_n-L}<\varepsilon\right].
\]	
\end{definition*}}
\begin{remark*}
	The real number $L\in\R$ is called \textbf{the limit}\footnote{The limit of a sequence is unique.}. When a sequence $\set{a_n}_{n=1}^\infty$ has the limit $L$, we will use the notation \[
	\lim_{n\to\infty}a_n=L\quad\text{or}\quad a_n\to L\ \text{as}\ n\to\infty.
	\]  That is, \[
		\lim_{n\to\infty}a_n=L\iff \forall\varepsilon>0:\exists N\in\N:\left[ n\geq N\implies \abs{a_n-L}<\varepsilon\right].
	\]
\end{remark*}
%\begin{remark*}
%		\\
%		&\iff\forall\varepsilon>0:\exists N(\varepsilon)\in\N:\left[ n\in[N(\varepsilon),\infty)\implies a(n)\in B_{\varepsilon}(L)\right] \\
%		&\iff \forall\varepsilon>0:\exists N(\varepsilon)\in\N:\left[ \set{a(n):n\in[N(\varepsilon),\infty)}\subseteq B_{\varepsilon}(L) \right]\\
%		&\iff\forall\varepsilon>0,\ \#\set{n\in\N: a_n\not\in(L-\varepsilon,L+\varepsilon)}<\infty.\\
%		&\iff \forall\varepsilon>0, a_n\in B_{\varepsilon}(L)\ \text{except some finite term.}
%	\end{align*}
%\end{remark*}

\newpage
\begin{note}
	If a sequence has a limit, we say that the sequence is \textbf{convergent}; if it has no limit, we say that the sequence is \textbf{divergent}.
\end{note}
\vfill
\begin{example*}
	Consider the sequence defined by $a_n=1/n$ for each $n\in\N$. Prove that \[
	\lim\limits_{n\to\infty}a_n=\lim\limits_{n\to\infty}\frac{1}{n}=0.
	\]
	\begin{center}
		\input{../tikz/grad-math-tikz/grad-math-4-exam1}
	\end{center}
	\begin{proof}
		\textcolor{blue}{Let $\varepsilon>0$}. By the Archimedean property, we obtain \[
		\textcolor{blue}{\exists N_\epsilon\in\N}\quad \text{s.t.}\quad 1<\varepsilon\cdot N_\epsilon,\ \ie,\ \frac{1}{N_\epsilon}<\varepsilon.
		\] \textcolor{blue}{Assume that $n\geq N_\varepsilon$ then} \[
		\textcolor{blue}{\abs{a_n-0}}=\abs{\frac{1}{n}}=\frac{1}{n}\leq\frac{1}{N_\varepsilon}
		\textcolor{blue}{<\varepsilon}.
		\] Hence $\displaystyle\lim\limits_{n\to\infty}\frac{1}{n}=0$.
	\end{proof}
\end{example*}
\vfill
\begin{example*}
	Consider the sequence defined by $b_n=1-(-1)^n$ for all $n\in\N$. Prove that $b_n$ does not converge. 
	\begin{center}
		\input{../tikz/grad-math-tikz/grad-math-4-exam2}
	\end{center}
	\begin{proof}
		The sequence $\set{b_n}$ alternates between $0$ and $2$: \[
		b_n=\begin{cases}
			0 &:n=2k \\
			2 &:n=2k+1
		\end{cases}
		\] with $k\in\N$.
		Suppose that $\set{b_n}_{n=1}^\infty$ converges to some limit $B\in\R$ and set
		$\varepsilon=1$. Then, by the definition of convergence:\[
		\exists N_\varepsilon\in\N\ \text{s.t.}\ n\geq N_\varepsilon\implies\abs{b_n-B}<1.
		\] \begin{enumerate}[(\text{Case} 1)]
			\item  For all even $n\geq N$, we have $b_n=0$.  Then the inequality $\abs{b_n-B}<1$ becomes \begin{equation}
				\abs{0-B}=\abs{B}<1,\ \ie, B\in(-1,1).
			\end{equation}
			\item For all odd $n\geq N$, we have $b_n=2$.  Then the inequality $\abs{b_n-B}<1$ becomes \begin{equation}
				\abs{2-B}<1,\ \ie,\ B\in\intoo{1,3}
			\end{equation}
		\end{enumerate}
		By (1) and (2), there is no intersection between these ranges; \[
		B\in(-1,1)\cap(1,3)=\varnothing
		\] which proves that $b_n$ does not converge.
		\begin{center}
			\input{../tikz/grad-math-tikz/grad-math-4-exam2-2}
		\end{center}
	\end{proof}
\end{example*}

%\begin{tikzpicture}[scale=1.5]
%	% Define constants for visualization
%	\def\N{5} % Example N_epsilon value
%	\def\yMax{3} % Max value for y-axis
%	\def\yMin{-1} % Min value for y-axis
%	
%	% Draw axes
%	\draw[thick,->] (0,0) -- (10,0) node[anchor=north] {$n$};
%	\draw[thick,->] (0,\yMin) -- (0,\yMax) node[anchor=east] {$b_n$};
%	
%	% Draw B regions
%	\draw[thick, blue] (0,1) -- (10,1) node[right] {$1$};
%	\draw[thick, blue] (0,-1) -- (10,-1) node[right] {$-1$};
%	\draw[thick, red] (0,3) -- (10,3) node[right] {$3$};
%	\draw[thick, red] (0,2) -- (10,2) node[right] {$2$};
%	
%	% Sequence points
%	\foreach \x in {1,...,9} {
%		\pgfmathsetmacro{\parity}{mod(\x,2) == 0 ? 0 : 2}
%		\filldraw (\x,\parity) circle (2pt);
%	}
%	
%	% Highlight the interval areas
%	\fill[blue, opacity=0.2] (0,-1) rectangle (10,1) node[pos=0.5, black, opacity=1] {$B \in (-1, 1)$};
%	\fill[red, opacity=0.2] (0,2) rectangle (10,3) node[pos=0.5, black, opacity=1] {$B \in (1, 3)$};
%	
%	% Annotations to explain the issue
%	\node at (5,0.5) [blue] {$B$ range for even $n$};
%	\node at (5,2.5) [red] {$B$ range for odd $n$};
%	\node at (5,\yMax) [black] {No intersection $\varnothing$};
%	
%\end{tikzpicture}
\newpage

\defbox[Absolute Value in Reals]{\begin{definition*}
	Let $x\in\R$. A \textbf{absolute value} $\abs{x}$ of $x$ is defined by \[
	\abs{x}:=\begin{cases}
		x &\text{if}\ x\geq 0\\
		-x &\text{if}\ x<0
	\end{cases}
	\]
\end{definition*}}
\begin{remark*}
	For $x\in\R$, \[
	\abs{x}=\begin{cases}
		x &:x>0 \\
		0 &:x=0\\
		-x &:x<0
	\end{cases}
	\]
\end{remark*}
\vfill
\probox[]{\begin{proposition}
Let $x,y\in\R$. \begin{enumerate}[\normalfont(1)]
	\item $\abs{x}=+\sqrt{x^2}$
	\item $\abs{x}\geq 0$
	\item $\abs{x}=0\Leftrightarrow x=0$
	\item $\abs{x}=\abs{-x}$
	\item $\abs{xy}=\abs{x}\abs{y}$
	\item (Fundamental Theorem of Absolute Values) For $c\geq 0$, we have \[
	\abs{x}\leq c\iff -c\leq x\leq c
	\]
	\item $-\abs{x}\leq x\leq\abs{x}$
\end{enumerate}
\end{proposition}}
\begin{proof}
\begin{enumerate}[(1)]
	\item If ($x\geq 0$) then $\abs{x}=x=\sqrt{x^2}$. Similarly if $x< 0$ then $\abs{x}=-x=\sqrt{x^2}$.
	\item $\abs{x}=\begin{cases}
		x\geq 0 &:x\geq 0\\
		-x>0 &:x<0
	\end{cases}\quad\geq 0$.
	\item[]
	\item \begin{itemize}
		\item[($\Leftarrow$)] If $x=0$ then $\abs{x}=x=0$.
		\item[($\Rightarrow$)] Let $\abs{x}=0$. Suppose that $x\neq0$. \begin{enumerate}[(i)]
			\item $x>0\implies \abs{x}=x>0\ \text{\Large\lightning}$
			\item $x<0\implies \abs{x}=-x>0\ \text{\Large\lightning}$
		\end{enumerate} Thus $x$ must be zero.
	\end{itemize}
	\newpage
	\item $\abs{-x}=\begin{cases}
		-x &: -x\geq 0\ (\ie, x\leq 0) \\
		-(-x)=x &: -x< 0\ (\ie, x> 0)
	\end{cases}=\begin{cases}
	x &\text{if}\ x\geq 0\\
	-x &\text{if}\ x<0
\end{cases}=\abs{x}$.
	\item $\abs{xy}=\begin{cases}
		xy=\abs{x}\abs{y} &:x\geq0,y\geq 0\\
		-xy=x(-y)=\abs{x}\abs{y} &:x\geq0,y< 0\\
		-xy=(-x)y=\abs{x}\abs{y} &:x<0,y\geq 0\\
		xy=(-x)(-y)=\abs{x}\abs{y} &:x<0,y< 0
	\end{cases}$
	\vspace{1cm}
	\item[\textcolor{red}{(6)}] 
	\begin{itemize}
		\item[($\Rightarrow$)] Let $\abs{x}\leq c$. \begin{enumerate}[(i)]
			\item $x\geq 0\implies x=\abs{x}\leq c$, \ie, $-c\leq 0\leq x\leq c$.
			\item $x<0\implies -x=\abs{x}\leq c$, \ie, $-c\leq x< 0\leq c$.
		\end{enumerate} Thus, $-c\leq x\leq c$.
		\vspace{.5cm}
		\item[($\Leftarrow$)] Let $-c\leq x\leq c$. \begin{enumerate}[(i)]
			\item $x\geq 0\implies \abs{x}=x\leq c$.
			\item $x<0\implies \abs{x}=-x\leq c$.
		\end{enumerate} Thus, $\abs{x}\leq c$.
	\end{itemize}
	\item[(7)] Let $c=\abs{x}$, where $c\geq 0$. By (6), thus, the result follows.
\end{enumerate}
\end{proof}
\vfill
\probox[Triangle Inequality]{\begin{proposition}
Let $x,y\in\R$. \begin{enumerate}[\normalfont(1)]
	\item $\abs{x+y}\leq\abs{x}+\abs{y}$
	\item $\abs{\abs{x}-\abs{y}}\leq\abs{x-y}$.
\end{enumerate}
\end{proposition}}
\begin{proof}
\begin{enumerate}[(1)]
	\item By (7) of \textbf{Proposition 1}, we have \[
	-\abs{x}\leq x\leq\abs{x},\quad-\abs{y}\leq y\leq\abs{y}.
	\] \newpage
	Then \begin{table}[h!]\centering\setstretch{1.5}
		\begin{tabular}{cccccc}
			&$-\abs{x}$ & $\leq$ & $x$ & $\leq$ & $\abs{x}$ \\
			+&$-\abs{y}$ & $\leq$ & $y$ & $\leq$ & $\abs{y}$ \\ \cline{2-6}
			&$-(\abs{x}+\abs{y})$& $\leq$& $x+y$&$\leq$& $\abs{x}+\abs{y}$ \\
		\end{tabular}
	\end{table}\\ Thus, we have $\abs{x+y}\leq\abs{x}+\abs{y}$.
	\item \ \begin{enumerate}[(i)]
		\item Note that \begin{align*}
			\abs{x} &=\abs{x-y+y} \\
			&\leq\abs{x-y}+\abs{y}\quad\text{by (1) of \textbf{Proposition 2}}
		\end{align*} Thus $\abs{x}-\abs{y}\leq\abs{x-y}$. 
		\item Note that \begin{align*}
			\abs{y}&=\abs{x-(x-y)}\\
			&\leq\abs{x}+\abs{-(x-y)}\quad\text{by (1) of \textbf{Proposition 2}} \\
			&=\abs{x}+\abs{x-y}\quad\text{by (4) of \textbf{Proposition 1}}
		\end{align*} Therefore $-\abs{x-y}\leq\abs{x}-\abs{y}$.
	\end{enumerate} By (i) and (ii), we know \[
	-\abs{x-y}\leq\abs{x}-\abs{y}\leq\abs{x-y},\quad\ie,\quad\abs{\abs{x}-\abs{y}}\leq\abs{x-y}.
	\]
\end{enumerate}
\end{proof}
\vfill
\defbox[Boundedness of Sequence]{\begin{definition*}
	Let $\set{a_n}_{n=1}^\infty(\subseteq\R)$ is a sequence. $\set{a_n}$ is said to be \textbf{bounded} if \[
		\exists M\in\R\ \text{such that}\ \forall n\in\N,\ \abs{a_n}\leq M.
		\]
\end{definition*}}

\newpage
\probox[]{\begin{proposition}
	A convergent sequence is bounded.
\end{proposition}}
\begin{proof}
	Let $\lim\limits_{n\to\infty}a_n=L$. By the definition of convergence, for $\varepsilon=1$,  \[
	\exists N\in\N\ \text{such that}\ n\geq N\implies\abs{a_n-L}<1.
	\] By triangle inequality, we have \[
	\abs{a_n}=\abs{a_n-L+L}\leq\abs{a_n-L}+\abs{L}<1+\abs{L}.
	\] Let $M:=\max\set{\abs{a_1},\abs{a_2},\dots,\abs{a_{N-1}},1+\abs{L}}$. Then \[
	\abs{a_n}\leq M
	\] for all $n\in\N$. Therefore $\set{a_n}$ is bounded.
\begin{center}
	\input{../tikz/grad-math-tikz/grad-math-4-conv-seq-bound}
\end{center}
\end{proof}
\vfill
\begin{note}
	We have established that if the limit of a sequence \(a_n\) exists as \(n\) approaches infinity, then there exists a real number \(M\) such that \(\lvert a_n \rvert \leq M\) for all \(n\): \[
	\exists A\in\R\ \text{s.t.}\ A=\lim_{n\to\infty}a_n\implies\exists M\in\R\ \text{s.t.}\ \forall n\in\N,\ \abs{a_n}\leq M.
	\]However, the converse is not necessarily true: \[
	\exists A\in\R\ \text{s.t.}\ A=\lim_{n\to\infty}a_n\centernot\impliedby\exists M\in\R\ \text{s.t.}\ \forall n\in\N,\ \abs{a_n}\leq M.
	\] To illustrate, consider the sequence \(\{a_n\} = 1 - (-1)^n\). This sequence is bounded, yet it does not converge, serving as a counterexample.
	\newpage
	Furthermore, we note the following important theorems:
	\begin{enumerate}
		\item \textbf{Monotone Convergence Theorem}:
		\begin{enumerate}[(i)]
			\item If a sequence \(\{a_n\}\) is bounded above and monotone increasing, then it converges.
			\item If a sequence \(\{a_n\}\) is bounded below and monotone decreasing, then it converges.
		\end{enumerate}
		\item \textbf{Bolzano-Weierstrass Theorem}: Every bounded sequence of real numbers has a convergent subsequence. That is, if there exists a real number \(M\) such that \(\lvert a_n \rvert < M\) for all \(n\), then there exists a convergent subsequence \(\{a_{n_k}\}\) of \(\{a_n\}\).
	\end{enumerate}
\end{note}

%\begin{tikzpicture}[scale=2]
%	\begin{axis}[
%		title=Example using the mesh parameter,
%		hide axis,
%		colormap/cool,
%		]
%		\addplot3[
%		mesh,
%		samples=50,
%		domain=-8:8,
%		]
%		{sin(deg(sqrt(x^2+y^2)))/sqrt(x^2+y^2)};
%		\addlegendentry{\(\frac{sin(r)}{r}\)}
%	\end{axis}
%\end{tikzpicture}
%\newpage
\vfill
\thmbox[Limit Theorem (Algebraic Property of Limit of Sequence)]{
\begin{theorem*} Let $\lim\limits_{n\to\infty}a_n=\alpha$, $\lim\limits_{n\to\infty}b_n=\beta$, and $k\in\R$. Then \begin{enumerate}[(1)]
		\item $\lim\limits_{n\to\infty}k a_n=k\lim\limits_{n\to\infty}a_n=k\alpha$.
		\item $\lim\limits_{n\to\infty}a_n\pm b_n=\lim\limits_{n\to\infty}a_n\pm\lim\limits_{n\to\infty}b_n=\alpha\pm\beta$.
		\item $\lim\limits_{n\to\infty}a_n b_n=\lim\limits_{n\to\infty}a_n\lim\limits_{n\to\infty}b_n=\alpha\beta$.
		\item $\displaystyle\lim\limits_{n\to\infty}\frac{a_n}{b_n}=\frac{\lim\limits_{n\to\infty}a_n}{\lim\limits_{n\to\infty}b_n}=\frac{\alpha}{\beta}$. (Here, $\beta\neq 0$ and $b_n\neq 0$)
%		\item $\lim\limits_{n\to\infty}\abs{a_n}=\abs{\lim\limits_{n\to\infty}a_n}=\abs{A}$.
%		\item $\lim\limits_{n\to\infty}(a_n)^p=A^p$. (Here, $p\in\N$).
%		\item $[\exists K:n\geq K\implies a_n\leq b_n]\implies A\leq B$.
	\end{enumerate}
\end{theorem*}}
\begin{proof}
	To be continue...
\end{proof}


\vfill
\begin{thebibliography}{9}
	\bibitem{advanced_calc_c}
	수학의 즐거움, Enjoying Math. ``수학 공부, 기초부터 대학원 수학까지, 6. 해석학 개론 (c) 수열의 수렴성.'' YouTube Video, 26:29. Published 
	September 20, 2019. URL: \url{https://www.youtube.com/watch?v=jwLfzJyIxmU}.
	\bibitem{advanced_calc_d}
	수학의 즐거움, Enjoying Math. ``수학 공부, 기초부터 대학원 수학까지, 7. 해석학 개론 (d) 극한 정리'' YouTube Video, 26:46. Published 
	September 26, 2019. URL: \url{https://www.youtube.com/watch?v=1TRD34QbIaw}.
\end{thebibliography}

%\newpage
%\appendix
\end{document}
