\documentclass[11pt,openany]{article}

\input{grad-math-preamble}
\input{tcolorbox}
\input{theorem}
\input{tikz}
\input{grad-math-commands}

\setstretch{1.25}
\begin{document}
\pagenumbering{arabic}
\begin{center}
	\huge\textbf{Set Theory}\\
	\vspace{0.5em}
	\large{Ji, Yong-hyeon}\\
	\vspace{0.5em}
	\normalsize{\today}\\
\end{center}

\section*{Terminology}

\begin{itemize}
	\item Set; Collection; Family.
	\item Tabular (or Roster) Form \[
	A=\set{0,2,4,8}.
	\]
	\item Set-builder Form \[
	A=\set{x:\ \text{is even and}\ x <10}.
	\]
\end{itemize}

\begin{example*}
	\ \begin{itemize}
		\item $\mathbb{N}=\set{1,2,\dots}$
		\item $\mathbb{Z}=\set{\dots,-2,-1,0,1,2,\dots}$
		\item $\mathbb{Q}=\set{\frac{p}{q}:p\in\mathbb{Z},q\in\mathbb{Z}\setminus\set{0}, \gcd(p,q)=1}$
		\item $\mathbb{R}=\set{x: x\ \text{is a real number}}$
		\item $\mathbb{C}=\set{z:z\ \text{is a complex number}}$
	\end{itemize}
\end{example*}
\vfill
\begin{exercise*}
	Show that $\sqrt{2}$ is irrational.
	\begin{proof}[\sol]
		\textcolor{gray!20!white}{Assume \( \sqrt{2} \in \mathbb{Q} \), i.e., \( \exists p, q \in \mathbb{Z} \) such that
		$\sqrt{2}q = p, \quad g\neq 0$ and $\gcd(p, q) = 1.$
		Then $2q^2 = p^2$. Since \( p^2 \) is even \( \Rightarrow p \) is even,
		\[
		p = 2k \quad \text{for some } k \in \mathbb{Z}
		\]
		By substituting \( p = 2k \) into \( 2q^2 = p^2 \), we have
		\[
		2q^2 = (2k)^2 \implies 2q^2 = 4k^2 \implies q^2 = 2k^2
		\]
		Since \( q^2 \) is even \( \Rightarrow q \) is even,
		\[
		q = 2m \quad \text{for some } m \in \mathbb{Z}
		\]
		Thus, \( p \) and \( q \) are both even \( \implies \gcd(p, q) \geq 2 \), which contradicts the assumption \( \gcd(p, q) = 1 \).}
	\end{proof}
\end{exercise*}

\newpage
\defbox[Subset and Set Equality]{\begin{definition*}
		Let $A$ and $B$ are sets.
		\begin{itemize}
			\item $B\subseteq A\overset{\text{def}}{\iff}(x\in B\Rightarrow x\in A)$.
			\item Set Equality: \begin{align*}
				A=B&\overset{\text{def}}{\iff} A\subseteq B\land B\subseteq A\\
				&\iff (x\in A\Rightarrow x\in B)\land(x\in B\Rightarrow x\in A).
			\end{align*}
		\end{itemize}
\end{definition*}}
\vfill
\defbox[Power Set]{\begin{definition*}
	The power set of a set $X$ is the set of all subsets of $X$.	
	\[
	\mathcal{P}(X)=2^X:=\set{S:S\subseteq X}.
	\]
\end{definition*}}
\vfill
\defbox[Cartesian Product]{\begin{definition*}
	Let $A$ and $B$ are sets. The \textbf{cartesian product} of $A$ and $B$ is the set \[
	A\times B=\set{(a,b):a\in A\land b\in B}.
	\]
\end{definition*}}
\vfill
\defbox[Union, Intersection and Complement]{\begin{definition*}
	Let $U$ is a universal set, and let $A,B\subseteq U$.
	\begin{itemize}
		\item The \textbf{union} of $A$ and $B$ is the set \[
		\boxed{A\cup B:=\set{x:x\in A\lor x\in B}}.
		\] Note that $x\in A\cup B\iff x\in A\lor x\in B$.
		\item The \textbf{intersection} of $A$ and $B$ is the set \[
		\boxed{A\cap B:=\set{x:x\in A\land x\in B}}.
		\] Note that $x\in A\cap B\iff x\in A\land x\in B$.
		\item The \textbf{complement} of $A$ is the set \[
		\boxed{A^C:=\set{x:\lnot(x\in A)}=\set{x:x\notin A}}.
		\] Note that $x\in A^C\iff x\notin A$.
	\end{itemize}
\end{definition*}}

\newpage

\probox[]{\begin{proposition}
	Let $A,B,C\subseteq U$.
	\begin{enumerate}[(1)]
		\item $A\cap(B\cup C)=(A\cap B)\cup(A\cap C)$.
		\item $A\cup(B\cap C)=(A\cup B)\cap(A\cup C)$.
		\item $(A\cup B)^C=A^C\cap B^C$.
		\item $(A\cap B)^C=A^C\cup B^C$.
	\end{enumerate}
\end{proposition}}
\begin{proof}
	\begin{enumerate}[(1)]
		\item 
		\item 
		\item \textcolor{gray!20!white}{$(A\cup B)^C=\set{x:\lnot\left[x\in A\lor x\in B\right]}=\set{x:x\notin A\land x\notin B}=A^C\cap B^C.$}
		\item \textcolor{gray!20!white}{$(A\cap B)^C=\set{x:\lnot\left[x\in A\land x\in B\right]}=\set{x:x\notin A\lor x\notin B}=A^C\cup B^C.$}
	\end{enumerate}
\end{proof}

\vfill
\begin{exercise*}
	Let $A$ has $n$ elements. Show that $\mathcal{P}(A)$ has $2^n$ elements.
	\begin{proof}[\sol] 
		\textcolor{gray!20!white}{\begin{itemize}
			\item[(pf 1)] For each element of $A$, there are two choices:
			\begin{enumerate}
				\item Include the element in the subset.
				\item Exclude the element from the subset.
			\end{enumerate}
			Since we have two independent choices (include or exclude), the total number of subsets is:
			\[
			\underbrace{2\times 2\times\cdots 2}_{n\ \text{times}}=2^n.
			\]
			\item[(pf 2)] We use mathematical induction.
			\ \\
			(Basic Step) Let $A=\varnothing$ (so $\abs{A}=0$). Then $\mathcal{P}(A)=\set{\varnothing}$ and so $\abs{\mathcal{P}(A)}=\abs{\set{\varnothing}}=1$.
			\ \\
			(Inductive Step) Assume that $\abs{\mathcal{P}(A)}=2^k$ where $\abs{A}=k$ for some $k\in\mathbb{Z}_{\geq  0}$. Let $A'=A\cup\set{x}$ where $\abs{A}=k$ and $x\notin A$. That is, $\abs{A'}=k+1$. Then \[
			\mathcal{P}(A')=\mathcal{P}(A)\cup\set{S\cup \set{x}:S\in \mathcal{P}(A)}.
			\] This implies $\abs{\mathcal{P}(A')}=\abs{\mathcal{P}(A)} + \abs{\mathcal{P}(A)}.$ Therefore, by assumption, $\abs{\mathcal{P}(A')}=2^k + 2^k=2^{k+1}.$
		\end{itemize}}
	\end{proof}
\end{exercise*}

\newpage
\defbox[Function]{\begin{definition*}
	Let $A$ and $B$ are sets. A $\textbf{function}$ $f\subseteq A\times B$ \textbf{from $\boldmath{A}$ to $\boldmath{B}$} is a relation on $A\times B$ satisfying as follows:
	\begin{enumerate}[(i)]
		\item Every element of $A$ relates to some element of $B$. \[\boxed{
		\forall a\in A:\exists b\in B\ \text{such that}\ (a,b)\in f.}
		\]
		\item Every element of $A$ relates to \underline{no more than one} element of its $B$.\[\boxed{
		\forall a\in A:\forall b_1,b_2\in B: (a,b_1),(a,b_2)\in f\implies b_1=b_2.}
		\]
	\end{enumerate}
\end{definition*}}
\begin{remark*}
	A relation $f\subseteq A\times B$ is a function if \[
	\boxed{\forall a\in A:\exists! b\in B:(a,b)\in f.}
	\]
	\begin{itemize}
		\item The \textbf{domain} of $f$ is $\text{Dom}(f)=A$.
		\item The \textbf{codomain} of $f$ is $\text{Cdm}(f)=B$.
		\item The \textbf{image} of $f$ is the set \begin{align*}\
			\img{f}=f[A]:&=\set{b\in B:\exists a \in A\ \text{s.t.}\ (a,b)\in f}\\
			&=\set{b\in B:\exists a \in A\ \text{s.t.}\ f(a)=b}\\
			&=\set{b\in B: b = f(a)\ \text{for some}\ a\in A}.
		\end{align*} Simply we can express it as $f[A]=\set{f(a)\in B:a\in A}$. Note that $f[A]\subseteq B=\text{Cdm}(f)$. 
	
		Note that \begin{align*}
			b\in f[A]\iff b=f(a)\ \text{for some}\ a\in A.
		\end{align*}
		\item The \textbf{preimage} of $f$ is the set \begin{align*}
			\preimg{f}=f^{-1}[B]:&=\set{a\in A:\exists b \in B\ \text{s.t.}\ b=f(a)}\\
			&=\set{a\in A:f(a)=b\ \text{for some}\ b\in B}.
		\end{align*} Simply we can express it as $f^{-1}[B]=\set{a\in A:f(a)\in B}$. Note that $f^{-1}[B]\subseteq A=\text{Dom}(f)$.
	
		Note that \begin{align*}
		a\in f^{-1}[B]\iff f(a)\in B.
\end{align*}
	\end{itemize}
\end{remark*}

\newpage
\probox{\begin{proposition}
	Let $f:A\to B$ be a function from $A$ to $B$, and let $A_1,A_2\subseteq A$. \begin{enumerate}[(1)]
		\item $f[A_1\cup A_2]=f[A_1]\cup f[A_2]$.
		\item $f[A_1\cap A_2]\subseteq f[A_1]\cap f[A_2]$.
	\end{enumerate}
\end{proposition}}
\begin{proof}
\ \textcolor{gray!20!white}
%\ \textcolor{black}
{Recall that \[
	b\in f[A]\iff b=f(a)\ \text{for some}\ a\in A.
	\]\begin{enumerate}[(1)]
	\item \begin{itemize}
		\item[($\subseteq$)] \underline{Let $b\in f[A_1\cup A_2]$}. By the definition of the image, $b=f(a)$ for some $a\in A_1\cup A_2$. Then, either $a\in A_1$ or $a\in A_2$. \\
		\ \\ (Case 1) $a\in A_1\Rightarrow f(a)\in f[A_1](\subseteq f[A_1]\cup f[A_2])$.
		\ \\ (Case 2) $a\in A_2\Rightarrow f(a)\in f[A_2](\subseteq f[A_1]\cup f[A_2])$.\\
		\ \\ \underline{Thus, $b=f(a)\in f[A_1]\cup f[A_2]$}, and so $f[A_1\cup A_2]\subseteq f[A_1]\cup f[A_2]$.
		\vspace{24pt}
		\item[($\supseteq$)] \underline{Let $b\in f[A_1]\cup f[A_2]$}. Then either $b\in f[A_1]$ or $b\in f[A_2]$. \\
		\ \\ (Case 1) $b\in f[A_1]\Rightarrow b=f(a_1)$ for some $a_1\in A_1$.
		\ \\ (Case 2) $b\in f[A_1]\Rightarrow b=f(a_2)$ for some $a_2\in A_2$. \\
		\ \\ That is, $\exists a\in A_1\cup A_2$ such that $f(a)=b$ and $a\in\set{a_1,a_2}$. \underline{Thus, $b\in f[A_1\cup A_2]$}.
	\end{itemize}
		\vspace{36pt}
		\item \underline{Let $b\in f[A_1\cap A_2]$}. By the definition of the image, $b=f(a)$ for some $a\in A_1\cap A_2$. Since $a\in A_1\cap A_2$, we have $a\in A_1$ and $a\in A_2$. Then \textit{both} of the following hold: \begin{enumerate}[(i)]
			\item $a\in A_1\implies f(a)\in f[A_1]$
			\item $a\in A_2\implies f(a)\in f[A_2]$
		\end{enumerate} \underline{Therefore, $b=f(a)\in f[A_1]\cap f[A_2]$}.
\end{enumerate}}
\end{proof}

\newpage
\probox{\begin{proposition}
	Let $f:A\to B$ be a function from $A$ to $B$, and let $B_1,B_2\subseteq B$. \begin{enumerate}[(1)]
		\item $f^{-1}[B_1\cup B_2]=f^{-1}[B_1]\cup f^{-1}[B_2]$.
		\item $f^{-1}[B_1\cap B_2]=f^{-1}[B_1]\cap f^{-1}[B_2]$.
		\item $f^{-1}[B_1^C]=(f^{-1}[B_1])^C$.
	\end{enumerate}
\end{proposition}}
\begin{proof}
\ \textcolor{gray!20!white}
%\textcolor{black}
{Recall that \[ a\in f^{-1}[B]\iff f(a)\in B.\]
	\begin{enumerate}[(1)]
	\item \begin{itemize}
		\item[($\subseteq$)] \underline{Let $a\in f^{-1}[B_1\cup B_2]$}. By the definition of the preimage, we have $f(a)\in B_1\cup B_2$. That is, either $f(a)\in B_1$ or $f(a)\in B_2$. \\
		\ \\ (Case 1) $f(a)\in B_1\implies a\in f^{-1}[B_1]$.
		\ \\ (Case 2) $f(a)\in B_2\implies a\in f^{-1}[B_2]$. \\
		\ \\ \underline{Thus, $a\in f^{-1}[B_1]\cup f[B_2]$}.
		\vspace{12pt}
		\item[($\supseteq$)] \underline{Let $a\in f^{-1}[B_1]\cup f^{-1}[B_2]$}. Then either $a\in f^{-1}[B_1]$ or $a\in f^{-1}[B_2]$. \\
		\ \\ (Case 1) $a\in f^{-1}[B_1]\implies f(a)\in B_1$.
		\ \\ (Case 2) $a\in f^{-1}[B_2]\implies f(a)\in B_2$. \\
		\ \\ That is, $f(a)\in B_1\cup B_2$. \underline{Thus, $a\in f^{-1}[B_1\cup B_2]$}.
	\end{itemize}
	\vspace{24pt}
	\item \begin{itemize}
		\item[($\subseteq$)] \underline{Let $a\in f^{-1}[B_1\cap B_2]$}. By the definition of the preimage, $
		f(a)\in B_1\cap B_2$ and so $f(a)\in B_1$ and $f(a)\in B_2$. Then \textit{both} of the following hold:\\ \begin{enumerate}[(i)]
			\item $f(a)\in B_1\implies a\in f^{-1}[B_1]$.
			\item $f(a)\in B_2\implies a\in f^{-1}[B_2]$.
		\end{enumerate}\ \\ \underline{Thus, $a\in f^{-1}[B_1]\cap f[B_2]$}.
		\vspace{12pt}
		\newpage
		\item[($\supseteq$)] \underline{Let $a\in f^{-1}[B_1]\cap f^{-1}[B_2]$}. Then $a\in f^{-1}[B_1]$ and $a\in f^{-1}[B_2]$. Then \textit{both} of the following hold:\\ \begin{enumerate}[(i)]
			\item $a\in f^{-1}[B_1]\implies f(a)\in B_1$.
			\item $a\in f^{-1}[B_2]\implies f(a)\in B_2$.
		\end{enumerate} \ \\
		That is, $f(a)\in B_1\cap B_2$. \underline{Thus, $a\in f^{-1}[B_1\cap B_2]$}.
	\end{itemize}
	\vspace{12pt}
	\item \begin{itemize}
		\item[($\subseteq$)] 
		\underline{Let $a\in f^{-1}[B_1^C]$}. By the definition of the preimage, thus, \[
		f(a)\in B_1^C\implies f(a)\notin B_1\implies a\notin f^{-1}[B_1]\implies a\in(f^{-1}[B_1])^C.
		\]
		\item[($\supseteq$)] Let $a\in(f^{-1}[B_1])^C$. By the definition of the preimage and the complement, thus, \[
		a\notin f^{-1}[B_1]\implies f(a)\notin B_1\implies f(a)\in B_1^C\implies a\in f^{-1}[B_1^C].
		\]
	\end{itemize}
\end{enumerate}}
\end{proof}
\vfill
\probox{\begin{proposition}
	Let $f:A\to B$ be a function from $A$ to $B$. Let $A_1\subseteq A$ and $B_1\subseteq B$. \begin{enumerate}[(1)]
		\item $f[f^{-1}[B_1]]\subseteq B_1$.
		\item $A_1\subseteq f^{-1}[f[A_1]]$.
	\end{enumerate}
\end{proposition}}
\begin{proof}
\textcolor{gray!20!white}{
	Recall that \[\begin{array}{ll}
		f^{-1}[B_1]:=\set{a\in A:f(a)\in B_1}, &\quad\quad f[A_1]:=\set{f(a)\in B:a\in A_1}, \\
		f[f^{-1}[B_1]]:=\set{f(a)\in B:a \in f^{-1}[B_1]}, &\quad\quad f^{-1}[f[A_1]]:=\set{a\in A:f(a)\in f[A_1]}.
	\end{array}\]\begin{enumerate}[(1)]
		\item \underline{Let $b \in f[f^{-1}[B_1]]$}. By the definition of the image, \[
		\exists a\in f^{-1}[B_1]\ \text{such that}\ b = f(a).
		\] From the definition of the preimage, $a\in f^{-1}[B_1]\Rightarrow f(a)\in B_1$. \underline{Thus $b=f(a)\in B_1$.}
		\vspace{12pt}
		\item \underline{Let $a\in A_1$.} By the definition of the image, we know that $f(a)\in f[A_1]$. By the definition of the preimage, $f(a)\in f[A_1]\Rightarrow \underline{a\in f^{-1}[f[A_1]]}$.
	\end{enumerate}}
\end{proof}

\begin{example*}[Counterexample]
	Consider a function $f:A\to B$, where $A=\set{1,2}$ and $B=\set{a,b}$.
	\begin{center}\begin{tikzpicture}
			% Draw the sets A and B
			\draw[thick] (-2,0) ellipse (1 and 2);
			\draw[thick] (2,0) ellipse (1 and 2);
			
			% Labels for sets
			\node at (-2, 2.25) {$A$};
			\node at (2, 2.25) {$B$};
			
			% Draw the arrows representing the function
			\draw[-Stealth, thick] (-1.5, 2.25) -- (1.5,2.25) node[midway, above] {$f$};
			
			\node at (-2, .75) {$1$};
			\node at (-2, -.75) {$2$};
			\draw[fill] (-1.75,.75) circle (.05);
			\draw[fill] (-1.75,-.75) circle (.05);
			
			\node at (2, .75) {$a$};
			\node at (2, -.75) {$b$};
			\draw[fill] (1.75,.75) circle (.05);
			\draw[fill] (1.75,-.75) circle (.05);
			
			\draw[-Stealth, thick] (-1.75, .75) -- (1.75, .75);
			\draw[-Stealth, thick] (-1.75, -.75) -- (1.75, .75);
		\end{tikzpicture}
	\end{center}
	\begin{enumerate}[(1)]
		\item Let $B_1=\set{b}\subseteq B$. Then \[
		f^{-1}[B_1]=\varnothing\implies f[f^{-1}[B]]=f[\varnothing]=\varnothing\neq \set{b}=B_1.
		\]
		\item Let $A_1=\set{1}\subseteq A$. Then \[
		f[A_1]=f[\set{1}]=\set{a}\implies f^{-1}[f[A_1]]=f^{-1}[\set{a}]=\set{1,2}\neq \set{1}=A_1.
		\]
	\end{enumerate}
\end{example*}
\vfill
\defbox[Injection and Surjection]{\begin{definition*}
	Let $f:A\to B$ is a function from $A$ to $B$. \begin{itemize}
		\item  A function $f$ is \textbf{an injection} or \textbf{injective} (or \textbf{one-to-one}) if and only if \[
		\boxed{\forall a_1,a_2\in A:[f(a_1)=f(a_2)\implies a_1=a_2].}
		\] That is, an \textbf{injection} is a mapping such that the output uniquely determines its input.
		\item A function $f$ is \textbf{a surjection} or \textbf{surjective} (or \textbf{onto}) if and only if \[
		\boxed{\forall b\in B:[\exists a \in A\ \text{such that}\ f(a)=b].}
		\] That is, a \textbf{surjection} is a mapping such that every element of $B$ is related to by some element of $A$.
	\end{itemize}
\end{definition*}}
\begin{remark*}
	A function $f$ is \textbf{bijective} if and only if $f$ is both injective and surjective.
\end{remark*}

\newpage
\defbox[Composition of Functions]{\begin{definition*}
	Let $f_1:A\to B$ and $f_2:B\to C$ be functions such that $\text{Cdm}(f_1)=B=\text{Dom}(f_2)$. The \textbf{composition} $f_2\circ f_1$ is defined as: \[
	(f_2\circ f_1)(a):= f_2(f_1(a)).
	\] for all $a\in A$.
\end{definition*}}
\begin{remark*}
\ \begin{itemize}
	\item $f_2\circ f_1=\set{(a,c)\in A\times C: (f_1(a), c)\in f_2}$.
	\item $f_2\circ f_1=\set{(a,c)\in A\times C: \exists b\in f_2\ \text{s.t.}\ f_1(a)=b\land f_2(b)=c}$.
\end{itemize}
\end{remark*}
\vfill
\begin{note}[Diagram]
\ \begin{figure}[h!]
	\centering
	\begin{tikzcd}
		A \arrow[rrr, "f_1"] \arrow[rrrddd, "f_2\circ f_1"', dashed] &  &  & B \arrow[ddd, "f_2"] \\
		&  &  &                        \\
		&  &  &                        \\
		&  &  & C                   
	\end{tikzcd}
%	\caption{Diagram of $f_2\circ f_1$}
\end{figure}
\end{note}
\vfill
\begin{note}[Illustration]
	\ \begin{center}\begin{tikzpicture}[scale=.9]
	% Draw the sets A, B and C
	\filldraw[thick, cyan!50] (-6,0) ellipse (2.75 and 4);
	\draw[thick, line width = .25mm] (-6,0) ellipse (2.75 and 4);
	\filldraw[thick, magenta!50] (0,0) ellipse (2.75 and 4);
	\draw[thick, line width = .25mm] (0,0) ellipse (2.75 and 4);
	\filldraw[thick, yellow!50] (6,0) ellipse (2.75 and 4);
	\draw[thick, line width = .25mm] (6,0) ellipse (2.75 and 4);
	
	\filldraw[thick, cyan!50] (0,0) ellipse (2 and 2.5);
	\draw[thick, line width = .25mm] (0,0) ellipse (2 and 2.5);
	
	\filldraw[thick, magenta!50] (6,0) ellipse (2.5 and 2.5);
	\draw[thick, line width = .25mm] (6,0) ellipse (2.5 and 2.5);
	\filldraw[thick, cyan!50] (6,0) ellipse (2.25 and 1);
	\draw[thick, line width = .25mm] (6,0) ellipse (2.25 and 1);
	
	% Draw the arrows representing the function
	\draw[-Stealth, thick] (-5.5, 4) -- (-.5,4) node[midway, above] {$f_1$};
	\draw[-Stealth, thick] (.5, 4) -- (5.5,4) node[midway, above] {$f_2$};
	
	% Labels for sets
	\node at (-6, 4.25) {$A$};
	\node at (0, 4.25) {$B$};
	\node at (6, 4.25) {$C$};
	\node at (-6, -4.5) {$\text{Dom}(f_1)$};
	\node at (0, -4.5) {$\text{Cdm}(f_1)=\text{Dom}(f_2)$};
	\node at (6, -4.5) {$\text{Cdm}(f_2)$};
	
	\node at (0, 0) {$\img{f_1}=f_1[A]$};
	\draw[dashed, thick, line width= .5mm, color=cyan] (-5.75, 4) -- (.25, 2.5);
	\draw[dashed, thick, line width= .5mm, color=cyan] (-5.75, -4) -- (.25, -2.5);
	
	\node at (6, 1.5) {$\img{f_2}=f_2[B]$};
	\draw[dashed, thick, line width= .5mm, color=magenta] (0.25, 4) -- (6.25, 2.5);
	\draw[dashed, thick, line width= .5mm, color=magenta] (0.25, -4) -- (6.25, -2.5);
	
	\node at (6, 0) {$\img{f_2\circ f_1}=f_2[f_1[A]]$};
	\draw[dashed, thick, line width= .5mm, color=cyan] (0.25, 2.5) -- (6.25, 1);
	\draw[dashed, thick, line width= .5mm, color=cyan] (0.25, -2.5) -- (6.25, -1);

\end{tikzpicture}
	\end{center}
\end{note}

\thmbox[]{\begin{theorem}
	Let $A$ and $B$ are sets. Let $f:A\to B$ be a function, and let $\textnormal{id}_A:A\to A$ and $\textnormal{id}_B$ are identity functions on $A$ and $B$, respectively.
	\begin{enumerate}[(1)]
		\item $f$ is one-to-one if and only if there exists the function $g:B\to A$ such that $g\circ f =\textnormal{id}_A$.
		\item $f$ is onto if and only if there exists the function $g:B\to A$ such that $f\circ g =\textnormal{id}_B$.
	\end{enumerate}
\end{theorem}}
\begin{remark*}
\ \begin{enumerate}[(1)]
	\item % https://tikzcd.yichuanshen.de/#N4Igdg9gJgpgziAXAbVABwnAlgFyxMJZABgBpiBdUkANwEMAbAVxiRAEEQBfU9TXfIRQAmclVqMWbAELdeIDNjwEiAFjHV6zVog7dxMKAHN4RUADMAThAC2SMiBwQkARk2SdIc3IvW7iN0dnRFEJbTYjHy8-e2onJFCAIxgwKCQAWgBmBwY6ZIYABX5lIRBLLCMACxwQd3DdIwAdRoBjLEsWgAJzToBeTuacGAAPHEhLG0ZgLCguAH1OLgouIA
	\begin{tikzcd}
		A \arrow[rr, "f"] \arrow[rrrr, "g\circ f = \textnormal{id}_A"', bend right] &  & B \arrow[rr, "g"] &  & A
	\end{tikzcd}
	\item % https://tikzcd.yichuanshen.de/#N4Igdg9gJgpgziAXAbVABwnAlgFyxMJZABgBpiBdUkANwEMAbAVxiRACEQBfU9TXfIRQAmclVqMWbAILdeIDNjwEiAFjHV6zVog7dxMKAHN4RUADMAThAC2SMiBwQkARk2SdII3IvW7iN0dnRFEJbTZzHxArW3tqJyRQgCMYMCgkAFoAZgcGOhSGAAV+ZSEQSywjAAscEHdw3XMAHSaAYyxLVoACIy6AXi6WnBgADxxISxtGYCwoLgB9Ti4KLiA
	\begin{tikzcd}
		B \arrow[rr, "g"] \arrow[rrrr, "f\circ g = \textnormal{id}_B"', bend right] &  & A \arrow[rr, "f"] &  & B
	\end{tikzcd}
\end{enumerate}
\end{remark*}
\begin{proof}
\begin{enumerate}[(1)]
	\item \begin{itemize}
		\item[($\Rightarrow$)] Assume that $f:A\to B$ is injective. We need to construct a function $g:B\to A$ such that $g\circ f=\textnormal{id}_A$.
	\end{itemize}
	\item 
\end{enumerate}
\end{proof}


\end{document}
